theories/Relational/GenericRulesComplex.v
@@ -3,7 +3,7 @@ From Coq Require FunctionalExtensionality.
 From Mon Require Export Base.
 From Mon.SRelation Require Import SRelation_Definitions SMorphisms.
 From Mon.sprop Require Import SPropBase SPropMonadicStructures.
-From Relational Require Import Category RelativeMonads RelativeMonadExamples Rel.
+From Relational Require Import OrderEnrichedCategory OrderEnrichedRelativeMonadExamples Rel.
 
 Set Primitive Projections.
 Set Universe Polymorphism.
@@ -16,13 +16,19 @@ Section RelationalProgramLogicFromRelativeMonad.
 
   (* The context takes all components of a (full) relational specification monad *)
 
-  Context (M1 M2 : Monad) (M12 := compPair M1 M2).
-  Context (W10 W20 : OrderedMonad)
-          (W1 := ordmonad_to_relmon W10)
-          (W2 := ordmonad_to_relmon W20).
-  Context (θ10 : MonadMorphism M1 W10) (θ20 : MonadMorphism M2 W20)
-          (θ1 := mmorph_to_rmmorph θ10) (θ2 := mmorph_to_rmmorph θ20).
+  (* Basic setup for each side: computational monad, unary specification monad
+  and an effect observation relating these *)
+  Context (M1 M2 : Monad) (W10 W20 : OrderedMonad)
+          (θ10 : MonadMorphism M1 W10) (θ20 : MonadMorphism M2 W20).
 
+  Let M12 := compPair M1 M2.
+  Let W1 := ordmonad_to_relmon W10.
+  Let W2 := ordmonad_to_relmon W20.
+  Let θ1 := mmorph_to_rmmorph θ10.
+  Let θ2 := mmorph_to_rmmorph θ20.
+
+
+  (* Now, we want a relational lifting of W1 × W2 *)
   Context (W0 : TypeCatSq -> OrdCat) (η : forall A, OrdCat⦅Jprod A;W0 A⦆)
           (actW : forall {A1 A2 B1 B2},
               OrdCat⦅discr A1;W1 B1⦆ ->
@@ -30,80 +36,82 @@ Section RelationalProgramLogicFromRelativeMonad.
               OrdCat⦅Jprod ⟨A1,A2⟩; W0 ⟨B1,B2⟩⦆ ->
               OrdCat⦅W0 ⟨A1,A2⟩; W0 ⟨B1,B2⟩⦆).
   Context (actW_proper : forall {A1 A2 B1 B2},
-              Proper (sim _ ==> sim _ ==> sim _ ==> sim _) (@actW A1 A2 B1 B2)).
+              SProper (ord_cat_le _ s==> ord_cat_le _ s==> ord_cat_le _ s==> ord_cat_le _) (@actW A1 A2 B1 B2)).
   Context (HW_law1 : forall A1 A2, actW _ _ _ _
-                                 (relmon_unit W1 A1)
-                                 (relmon_unit W2 A2)
-                                 (η ⟨A1,A2⟩) ∼ Id _).
+                                 (ord_relmon_unit W1 A1)
+                                 (ord_relmon_unit W2 A2)
+                                 (η ⟨A1,A2⟩) = Id _).
   Context (HW_law2 : forall A1 A2 B1 B2 f1 f2 f,
-              actW A1 A2 B1 B2 f1 f2 f ∙ η _ ∼ f).
+              actW A1 A2 B1 B2 f1 f2 f ∙ η _ = f).
   Context (HW_law3 : forall A1 A2 B1 B2 C1 C2 f1 f2 f g1 g2 g,
               actW A1 A2 C1 C2
-                   (relmon_bind W1 g1 ∙ f1)
-                   (relmon_bind W2 g2 ∙ f2)
+                   (ord_relmon_bind W1 g1 ∙ f1)
+                   (ord_relmon_bind W2 g2 ∙ f2)
                    (actW B1 B2 C1 C2 g1 g2 g ∙ f)
-                   ∼ (actW B1 B2 C1 C2 g1 g2 g) ∙ (actW A1 A2 B1 B2 f1 f2 f)).
+                   = (actW B1 B2 C1 C2 g1 g2 g) ∙ (actW A1 A2 B1 B2 f1 f2 f)).
   Context (actW_mon : forall A1 A2 B1 B2 f1 f1' f2 f2' f f',
-              f1 ≼ f1' -> f2 ≼ f2' -> f ≼ f' ->
-              actW A1 A2 B1 B2 f1 f2 f ≼ actW A1 A2 B1 B2 f1' f2' f').
+              f1 ⪷ f1' -> f2 ⪷ f2' -> f ⪷ f' ->
+              actW A1 A2 B1 B2 f1 f2 f ⪷ actW A1 A2 B1 B2 f1' f2' f').
   Import SPropNotations.
 
   (* We show that we can define the sur-approximation of this coq-development from that data *)
 
-  Program Definition W : RelationalSpecMonad :=
-    mkRelativeMonad (fun A => ⟨⟨W1 (nfst A), W2 (nsnd A)⟩, W0 A⟩)
-                    (fun A => ⟨⟨relmon_unit W1 (nfst A), relmon_unit W2 (nsnd A)⟩,
+  Program Definition W : preRelationalSpecMonad :=
+    mkOrdRelativeMonad (fun A => ⟨⟨W1 (nfst A), W2 (nsnd A)⟩, W0 A⟩)
+                    (fun A => ⟨⟨ord_relmon_unit W1 (nfst A), ord_relmon_unit W2 (nsnd A)⟩,
                            η A⟩)
                     (fun A B f =>
-                       ⟨⟨relmon_bind W1 (nfst (nfst f)),
-                         relmon_bind W2 (nsnd (nfst f))⟩,
+                       ⟨⟨ord_relmon_bind W1 (nfst (nfst f)),
+                         ord_relmon_bind W2 (nsnd (nfst f))⟩,
                        actW _ _ _ _ (nfst (nfst f)) (nsnd (nfst f)) (nsnd f)⟩)
                     _ _ _ _.
   Next Obligation.
     cbv ; intuition.
-    rewrite (funext H)=> //.
-    rewrite (funext H2)=> //.
-    congr (Spr1 (actW _ _ _ _ _ _ _) _); apply Ssig_eq ; apply funext=> //.
+    1-2:apply omon_bind; [sreflexivity| cbv=> ? ; auto].
+    apply: actW_mon=> ?; [apply p0| apply q0| apply q].
   Qed.
   Next Obligation.
-    intuition; [refine (relmon_law1 W1 _ _)
-               |refine (relmon_law1 W2 _ _)
-               |apply HW_law1].
+    f_equal ; [f_equal|]; rewrite ?HW_law1 //;
+      apply Ssig_eq ;apply: funext=> a /=; apply: monad_law2.
   Qed.
   Next Obligation.
-    intuition; [refine (relmon_law2 W1 _ _ _ _)
-               |refine (relmon_law2 W2 _ _ _ _)
-               |apply HW_law2].
+    move: f => [[f1 f2] frel].
+    f_equal ; [f_equal|] ; apply Ssig_eq.
+    1-2:apply: funext=> a /=; apply: monad_law1.
+    apply (f_equal Spr1). apply: HW_law2.
   Qed.
   Next Obligation.
-    intuition; [refine (relmon_law3 W1 _ _ _ _ _ _)
-               |refine (relmon_law3 W2 _ _ _ _ _ _)
-               |apply HW_law3].
+    f_equal ; [f_equal|] ; apply Ssig_eq.
+    1-2: apply: funext=> a /=; rewrite /bind monad_law3 //.
+    apply (f_equal Spr1). apply: HW_law3.
   Qed.
 
   Context (θW : forall {A}, OrdCat⦅Jprod (M12 A);W0 A⦆).
   Context (HθW_law1 : forall {A},
-              θW _ ∙ fmap Jprod (relmon_unit M12 A)
-                 ∼ η A).
+              θW _ ∙ ofmap Jprod (ord_relmon_unit M12 A)
+                 = η A).
   Context (HθW_law2 : forall {A B} (f:TypeCatSq⦅A;M12 B⦆),
-              θW _ ∙ fmap Jprod (relmon_bind M12 f)
-                 ∼ actW _ _ _ _
-                         (θ1 _ ∙ fmap discr (nfst f))
-                         (θ2 _ ∙ fmap discr (nsnd f))
-                         (θW _ ∙ fmap Jprod f) ∙ θW _).
+              θW _ ∙ ofmap Jprod (ord_relmon_bind M12 f)
+                 = actW _ _ _ _
+                         (θ1 _ ∙ ofmap discr (nfst f))
+                         (θ2 _ ∙ ofmap discr (nsnd f))
+                         (θW _ ∙ ofmap Jprod f) ∙ θW _).
 
-  Program Definition θ : RelationalEffectObservation M1 M2 W :=
-    mkRelMonMorph _ _ _ _ (fun A => ⟨⟨θ1 (nfst A), θ2 (nsnd A)⟩, θW A⟩) _ _.
+  Program Definition θ : preRelationalEffectObservation M1 M2 W :=
+    mkpreREO M1 M2 W (fun A => ⟨⟨θ1 (nfst A), θ2 (nsnd A)⟩, θW A⟩) _ _.
   Next Obligation.
-    intuition; [apply (rmm_law1 _ _ _ _ θ1)
-               |apply (rmm_law1 _ _ _ _ θ2)
-               |apply HθW_law1].
+    f_equal ; [f_equal|]; apply Ssig_eq ; apply: (f_equal Spr1).
+    apply (rmm_law1 _ _ _ _ θ1).
+    apply (rmm_law1 _ _ _ _ θ2).
+    apply HθW_law1.
   Qed.
   Next Obligation.
-    intuition; [apply (rmm_law2 _ _ _ _ θ1) |apply (rmm_law2 _ _ _ _ θ2)|].
-    move: (HθW_law2 _ _ ⟨nfst, nsnd⟩ ⟨nfst0, nsnd0⟩)=> /= -> //.
+    f_equal ; [f_equal|]; apply Ssig_eq ; apply: (f_equal Spr1).
+    apply (rmm_law2 _ _ _ _ θ1).
+    apply (rmm_law2 _ _ _ _ θ2).
+    apply: HθW_law2.
   Qed.
-  
+
 
   Import RelNotations.
 
@@ -123,6 +131,7 @@ Section RelationalProgramLogicFromRelativeMonad.
   (* And we prove the rule for binding computations *)
 
   Import SPropNotations.
+  Arguments actW {_ _ _ _} _ _ _.
   Lemma full_seq_rule {A1 A2 B1 B2}
         {m1 : M1 A1} {m2 : M2 A2} {wm1 wm2 wm}
         {f1 : A1 -> M1 B1} {f2 : A2 -> M2 B2}
@@ -130,30 +139,42 @@ Section RelationalProgramLogicFromRelativeMonad.
         {wf : OrdCat⦅Jprod ⟨A1,A2⟩ ; W0 ⟨B1, B2⟩⦆} :
     ⋅⊫ m1 ≈ m2 [{ wm1, wm2, wm }] ->
     (⦑A1,A2|fun=>fun=>unit|TyRel⦒ ⊫ f1 ≈ f2 [{ wf1, wf2,  wf }]) ->
-    ⋅⊫ bind m1 f1 ≈ bind m2 f2 [{ Spr1 (relmon_bind W1 wf1) wm1,
-                                  Spr1 (relmon_bind W2 wf2) wm2,
-                                  Spr1 (actW _ _ _ _ wf1 wf2 wf) wm }].
+    ⋅⊫ bind m1 f1 ≈ bind m2 f2 [{ wm1 ≫= wf1,
+                                  wm2 ≫= wf2,
+                                  (actW wf1 wf2 wf)∙1 wm }].
   Proof.
     intros [[Hm1 Hm2] Hm] [[Hf1 Hf2] Hf].
-    move: (rmm_law2 _ _ M12 W θ _ _ (to_prod f1 f2)) => /= [[-> ->] H12] ; intuition.
+    move: (rmm_law2 _ _ M12 W θ _ _ (to_prod f1 f2))=> /= [[H1 H2] H12].
+    intuition.
+    move: (f_equal (fun h => h m1) H1)=> /= ->.
     apply omon_bind=> //; apply (Hm1 tt).
+    move: (f_equal (fun h => h m2) H2)=> /= ->.
     apply omon_bind=> //; apply (Hm2 tt).
-    rewrite (H12 ⟨m1, m2⟩).
-    
+    move: (f_equal (fun h => h ⟨m1, m2⟩) H12) => /= -> //=.
     estransitivity.
     simpl in Hf1.
-    unfold ordcattr_hom_ord in Hf1.
     refine (actW_mon A1 A2 B1 B2
-                    (θ1 _ ∙ fmap discr f1) wf1
-                    (θ2 _ ∙ fmap discr f2) wf2
-                    (θW _ ∙ fmap Jprod (to_prod f1 f2)) wf
+                    (θ1 _ ∙ ofmap discr f1) wf1
+                    (θ2 _ ∙ ofmap discr f2) wf2
+                    (θW _ ∙ ofmap Jprod (to_prod f1 f2)) wf
                     _ _ _ _).
     move=> ? ; apply Hf1.
     move=> ? ; apply Hf2.
     move=> [? ?] /=; eapply (Hf ⦑ _ , _ | tt⦒).
-    eapply (Spr2 (actW _ _ _ _ _ _ _))=> //.
+    eapply (Spr2 (actW _ _ _))=> //.
     apply (Hm ⦑tt,tt|I⦒).
   Qed.
+
+  Import RelNotations.
+
+  (* Definition bindStrongRSM {Γ A1 A2 B1 B2} *)
+  (*            (wm1 : πl Γ -> W1 A1) *)
+  (*            (wm2 : πr Γ -> W2 A2) *)
+  (*            (wmrel : ⟬Γ⟭ -> W A1 A2) *)
+  (*            (wf1 : πl Γ × A1 -> W1 B1) *)
+  (*            (wf2 : πr Γ × A2 -> W2 B2) *)
+  (*            (wfrel : ⟬extends Γ A1 A2⟭ -> W B1 B2) *)
+  (* : ⟬Γ⟭ -> Wrel B1 B2 *)
 
 
 End RelationalProgramLogicFromRelativeMonad.
